updated mainly for AFP style presentation

Infrastructure.thy
@@ -1,41 +1,57 @@
+section \<open>Infrastructures\<close>
+text \<open>The Isabelle Infrastructure framework supports the representation of infrastructures 
+as graphs with actors and policies attached to nodes. These infrastructures 
+are the {\it states} of the Kripke structure. 
+The transition between states is triggered by non-parametrized
+actions @{text \<open>get, move, eval, put\<close>} executed by actors. 
+Actors are given by an abstract type @{text \<open>actor\<close>} and a function 
+@{text \<open>Actor\<close>} that creates elements of that type from identities 
+(of type @{text \<open>string\<close>}). Policies are given by pairs of predicates 
+(conditions) and sets of (enabled) actions.\<close>
+subsection \<open>Actors, actions, and data labels\<close>
 theory Infrastructure
-imports AT "/Applications/Isabelle2018.app/Isabelle/src/HOL/Hoare/Hoare_Logic"
+imports AT 
 begin
-datatype action = get | move | eval |put
+datatype action = get | move | eval | put
+
 typedecl actor 
 type_synonym identity = string
-consts Actor :: "string => actor"
-type_synonym policy = "((actor => bool) * action set)"
+consts Actor :: "string \<Rightarrow> actor"
+type_synonym policy = "((actor \<Rightarrow> bool) * action set)"
 
 definition ID :: "[actor, string] \<Rightarrow> bool"
 where "ID a s \<equiv> (a = Actor s)"
-
-(* a simple definition of data and instantiating 
-the generic types of the Hoare logic to pairs of owner and data as 
-basic data type for specification. This enables the unique marking
-(modulo insider impersonation) of data within the system. 
-The manipulation of the data (using simple while language) can thus 
-be modelled but additionally taking the ownership into account. We use 
-eval below and anchor the access control in restricing base functions
-for the basic com type *)
+text \<open>The Decentralised Label Model (DLM) \cite{ml:98} introduced the idea to
+label data by owners and readers. We pick up this idea and formalize
+a new type to encode the owner and the set of readers as a pair.
+The first element is the owner of a data item, the second one is the
+set of all actors that may access the data item.
+This enables the unique security 
+labelling of data within the system additionally taking the ownership into 
+account.\<close>
 type_synonym data = nat  
-  (* Inspired by Myers DLM mode: first is the owner of a data item, second is the
-     set of all actors that may access the data item *)
 type_synonym dlm = "actor * actor set"
-  (* the following type constructors are from Hoare_logic:
-     bexp and assn are just synonyms for set, and
-     com is a simple datatype repesenting while command language
-     over some basic 'a \<Rightarrow> 'a functions, while 'a sem is
-     just the type of relations 'a \<Rightarrow> 'a \<Rightarrow> bool representing relational
-     semantics *)
-type_synonym acond = "(dlm * data) bexp"
-type_synonym aassn = "(dlm * data) assn"
-type_synonym acom = "(dlm * data) com"
-type_synonym asem = "(dlm * data) sem"
-  
+
+subsection \<open>Infrastructure graphs and policies\<close>
+text\<open>Actors are contained in an infrastructure graph. An @{text \<open>igraph\<close>} contains
+a set of location pairs representing the topology of the infrastructure
+as a graph of nodes and a list of actor identities associated to each node 
+(location) in the graph.
+Also an @{text \<open>igraph\<close>} associates actors to a pair of string sets by
+a pair-valued function whose first range component is a set describing
+the credentials in the possession of an actor and the second component
+is a set defining the roles the actor can take on. More importantly in this 
+context, an  @{text \<open>igraph\<close>} assigns locations to a pair of a string that defines
+the state of the component and an element of type @{text \<open>(dlm * data) set\<close>}. This
+set of labelled data may represent a condition on that data.
+Corresponding projection functions for each of these components of an 
+@{text \<open>igraph\<close>} are provided; they are named @{text \<open>gra\<close>} for the actual set of pairs of
+locations, @{text \<open>agra\<close>} for the actor map, @{text \<open>cgra\<close>} for the credentials,
+and @{text \<open>lgra\<close>} for the state of a location and the data at that location.\<close>
 datatype location = Location nat
   datatype igraph = Lgraph "(location * location)set" "location \<Rightarrow> identity set"
-                         "actor \<Rightarrow> (string set * string set)"  "location \<Rightarrow> string * acond"
+                           "actor \<Rightarrow> (string set * string set)"  
+                           "location \<Rightarrow> string * (dlm * data) set"
 datatype infrastructure = 
          Infrastructure "igraph" 
                         "[igraph ,location] \<Rightarrow> policy set" 
@@ -48,7 +64,7 @@ primrec agra :: "igraph \<Rightarrow> (location \<Rightarrow> identity set)"
 where  "agra(Lgraph g a c l) = a"
 primrec cgra :: "igraph \<Rightarrow> (actor \<Rightarrow> string set * string set)"
 where  "cgra(Lgraph g a c l) = c"
-primrec lgra :: "igraph \<Rightarrow> (location \<Rightarrow> string * acond)"
+primrec lgra :: "igraph \<Rightarrow> (location \<Rightarrow> string * (dlm * data) set)"
 where  "lgra(Lgraph g a c l) = l"
 
 definition nodes :: "igraph \<Rightarrow> location set" 
@@ -57,13 +73,16 @@ where "nodes g == { x. (? y. ((x,y): gra g) | ((y,x): gra g))}"
 definition actors_graph :: "igraph \<Rightarrow> identity set"  
 where  "actors_graph g == {x. ? y. y : nodes g \<and> x \<in> (agra g y)}"
 
+text \<open>There are projection functions text{@ \<open>graphI\<close>} and text{@ \<open>delta\<close>} when applied
+to an infrastructure return the graph and the policy, respectively. Other projections
+are introduced for the labels, the credential, and roles and to express their meaning.\<close>
 primrec graphI :: "infrastructure \<Rightarrow> igraph"
 where "graphI (Infrastructure g d) = g"
 primrec delta :: "[infrastructure, igraph, location] \<Rightarrow> policy set"
 where "delta (Infrastructure g d) = d"
 primrec tspace :: "[infrastructure, actor ] \<Rightarrow> string set * string set"
   where "tspace (Infrastructure g d) = cgra g"
-primrec lspace :: "[infrastructure, location ] \<Rightarrow> string * acond"
+primrec lspace :: "[infrastructure, location ] \<Rightarrow> string * (dlm * data)set"
 where "lspace (Infrastructure g d) = lgra g"
 
 definition credentials :: "string set * string set \<Rightarrow> string set"
@@ -74,26 +93,29 @@ definition roles :: "string set * string set \<Rightarrow> string set"
   where  "roles lxl \<equiv> (snd lxl)"
 definition role :: "[igraph, actor * string] \<Rightarrow> bool"
   where "role G ac \<equiv> snd ac \<in> roles(cgra G (fst ac))"
-
 definition isin :: "[igraph,location, string] \<Rightarrow> bool" 
   where "isin G l s \<equiv> s = fst (lgra G l)"
 
+text \<open>Predicates and projections for the labels to encode their meaning.\<close>
 definition owner :: "dlm * data \<Rightarrow> actor" where "owner d \<equiv> fst(fst d)"
-    
-definition owns :: "[igraph, location, actor, dlm * data] \<Rightarrow> bool"    
+definition owns :: "[igraph, location, actor, dlm * data] \<Rightarrow> bool"
   where "owns G l a d \<equiv> owner d = a"
-    
 definition readers :: "dlm * data \<Rightarrow> actor set"
   where "readers d \<equiv> snd (fst d)"
 
+text \<open>The predicate @{text \<open>has_access\<close>} is true for owners or readers.\<close> 
 definition has_access :: "[igraph, location, actor, dlm * data] \<Rightarrow> bool"    
 where "has_access G l a d \<equiv> owns G l a d \<or> a \<in> readers d"
-  
+
+(*
+text \<open>Actors can delete data.\<close>
 definition actor_can_delete ::   "[infrastructure, actor, location] \<Rightarrow> bool"
 where actor_can_delete_def: "actor_can_delete I h l \<equiv>  
                    (\<forall> as n. ((h, as), n) \<notin> (snd (lgra (graphI I) l)))"
-        
-(* type of functions that preserves the security labeling *)    
+*)
+
+text \<open>We define a type of functions that preserves the security labeling and a 
+   corresponding function application  operator.\<close>  
 typedef label_fun = "{f :: dlm * data \<Rightarrow> dlm * data. 
                         \<forall> x:: dlm * data. fst x = fst (f x)}"  
 proof (auto)
@@ -104,10 +126,9 @@ qed
 
 definition secure_process :: "label_fun \<Rightarrow> dlm * data \<Rightarrow> dlm * data" ("_ \<Updown> _" 50)
   where "f  \<Updown> d \<equiv> (Rep_label_fun f) d" 
-    
-definition valid_proc :: "acond \<Rightarrow> label_fun \<Rightarrow> acond \<Rightarrow> bool"    
-  where "valid_proc a f b \<equiv> Valid a (Basic (Rep_label_fun f)) b"
-    
+
+(* This part is relevant to model Insiders but is not needed for Infrastructures.
+
 datatype psy_states = happy | depressed | disgruntled | angry | stressed
 datatype motivations = financial | political | revenge | curious | competitive_advantage | power | peer_recognition
 
@@ -136,24 +157,41 @@ where "Insider a C \<equiv> (tipping_point (astate a) \<longrightarrow> (\<foral
 
 definition Insider' :: "[actor \<Rightarrow> bool, identity, identity set] \<Rightarrow> bool" 
 where "Insider' P a C \<equiv> (tipping_point (astate a) \<longrightarrow> (\<forall> b\<in>C. UasI' P a b \<and> inj_on Actor C))"
+*)
 
+text \<open>The predicate atI -- mixfix syntax @{text \<open>@\<^bsub>G\<^esub>\<close>} -- expresses that an actor (identity) 
+      is at a certain location in an igraph.\<close>
 definition atI :: "[identity, igraph, location] \<Rightarrow> bool" ("_ @\<^bsub>(_)\<^esub> _" 50)
 where "a @\<^bsub>G\<^esub> l \<equiv> a \<in> (agra G l)"
 
+text \<open>Policies specify the expected behaviour of actors of an infrastructure. 
+They are defined by the @{text \<open>enables\<close>} predicate:
+an actor @{text \<open>h\<close>} is enabled to perform an action @{text \<open>a\<close>} 
+in infrastructure @{text \<open>I\<close>}, at location @{text \<open>l\<close>}
+if there exists a pair @{text \<open>(p,e)\<close>} in the local policy of @{text \<open>l\<close>}
+(@{text \<open>delta I l\<close>} projects to the local policy) such that the action 
+@{text \<open>a\<close>} is a member of the action set @{text \<open>e\<close>} and the policy 
+predicate @{text \<open>p\<close>} holds for actor @{text \<open>h\<close>}.\<close>
 definition enables :: "[infrastructure, location, actor, action] \<Rightarrow> bool"
 where
 "enables I l a a' \<equiv>  (\<exists> (p,e) \<in> delta I (graphI I) l. a' \<in> e \<and> p a)"
 
-(* behaviour is the good behaviour, i.e. everything allowed by policy *)
+text \<open>The behaviour is the good behaviour, i.e. everything allowed by the policy of infrastructure I.\<close>
 definition behaviour :: "infrastructure \<Rightarrow> (location * actor * action)set"
 where "behaviour I \<equiv> {(t,a,a'). enables I t a a'}"
 
-(* Most general: misbehaviour is the complement of behaviour *)
+text \<open>The misbehaviour is the complement of the behaviour of an infrastructure I.\<close>
 definition misbehaviour :: "infrastructure \<Rightarrow> (location * actor * action)set"
 where "misbehaviour I \<equiv> -(behaviour I)"
 
-(* state transition on infrastructures *)
+subsection "State transition on infrastructures"
+text \<open>The state transition defines how actors may act on infrastructures through actions
+    within the boundaries of the policy. It is given as an inductive definition over the 
+    states which are infrastructures.  This state transition relation is dependent on actions but also on
+    enabledness and the current state of the infrastructure.
 
+    First we introduce some auxiliary functions dealing
+    with repetitions in lists and actors moving in an igraph.\<close>
 primrec jonce :: "['a, 'a list] \<Rightarrow> bool"
 where
 jonce_nil: "jonce a [] = False" |
@@ -186,7 +224,6 @@ where
          \<rbrakk> \<Longrightarrow> I \<rightarrow>\<^sub>n I'"
 | get_data : "G = graphI I \<Longrightarrow> a @\<^bsub>G\<^esub> l \<Longrightarrow>
         enables I l' (Actor a) get \<Longrightarrow> 
-(* naive version omits the following two checks of the DLM labels *)
        ((Actor a', as), n) \<in> snd (lgra G l') \<Longrightarrow> Actor a \<in> as \<Longrightarrow> 
         I' = Infrastructure 
                    (Lgraph (gra G)(agra G)(cgra G)
@@ -217,11 +254,11 @@ where
                           ((lgra G)(l := (s, snd (lgra G l) \<union> {((Actor a, as), n)}))))
                    (delta I)
           \<Longrightarrow> I \<rightarrow>\<^sub>n I'"
-  
-    
+
+text \<open>Note that the type infrastructure can now be instantiated to the axiomatic type class 
+      @{text\<open>state\<close>} which enables the use of the underlying Kripke structures and CTL.\<close>
 instantiation "infrastructure" :: state
 begin
-
 definition 
    state_transition_infra_def: "(i \<rightarrow>\<^sub>i i') =  (i \<rightarrow>\<^sub>n (i' :: infrastructure))"
 
