GDPRhealthcare.thy
@@ -1,7 +1,22 @@
+section \<open>Application example from IoT healthcare\<close> 
+text \<open>The  example of an IoT healthcare systems is taken from the context of the CHIST-ERA project
+SUCCESS \cite{suc:16}.  In this system architecture, data is collected by sensors 
+in the home or via a smart phone helping to monitor bio markers of the patient. The data 
+collection is in a cloud based server to enable hospitals (or scientific institutions) 
+to access the data which is controlled via the smart phone.
+The identities Patient and Doctor represent patients
+and their doctors; double quotes ''s'' indicate strings 
+in Isabelle/HOL.
+The global policy is `only the patient and the doctor can access the data in the cloud'.\<close>
 theory GDPRhealthcare
 imports Infrastructure
 begin
-
+text \<open>Local policies are represented as a function over an @{text \<open>igraph G\<close>} 
+      that additionally assigns each location of a scenario to its local policy 
+      given as a pair of requirements to an actor (first element of the pair) in 
+      order to grant him actions in the location (second element of the pair). 
+      The predicate @{text \<open>@G\<close>} checks whether an actor is at a given location 
+       in the @{text \<open>igraph G\<close>}.\<close>
 locale scenarioGDPR = 
 fixes gdpr_actors :: "identity set"
 defines gdpr_actors_def: "gdpr_actors \<equiv> {''Patient'', ''Doctor''}"
@@ -33,12 +48,10 @@ defines ex_creds_def: "ex_creds \<equiv> (\<lambda> x. if x = Actor ''Patient'' 
                             (if x = Actor ''Doctor'' then
                                 ({''PIN''},{}) else ({},{})))"
 
-
-fixes ex_locs :: "location \<Rightarrow> string * acond"
+fixes ex_locs :: "location \<Rightarrow> string * (dlm * data) set"
 defines "ex_locs \<equiv> (\<lambda> x.  if x = cloud then
              (''free'',{((Actor ''Patient'',{Actor ''Doctor''}),42)}) 
              else ('''',{}))"
-
 
 fixes ex_loc_ass :: "location \<Rightarrow> identity set"
 defines ex_loc_ass_def: "ex_loc_ass \<equiv>
@@ -47,15 +60,14 @@ defines ex_loc_ass_def: "ex_loc_ass \<equiv>
                        else {}))"
 
 (* The nicer representation with case suffers from
-   not so nice presentation in the cases (need to unfold the syntax) *) 
+   not so nice presentation in the cases (need to unfold the syntax)  
 fixes ex_loc_ass_alt :: "location \<Rightarrow> identity set"
 defines ex_loc_ass_alt_def: "ex_loc_ass_alt \<equiv>
           (\<lambda> x.  (case x of 
              Location (Suc 0) \<Rightarrow> {''Patient''}  
            | Location (Suc (Suc 0)) \<Rightarrow> {''Doctor'', ''Eve''} 
            |  _ \<Rightarrow> {}))"
-  
-
+*)
 fixes ex_graph :: "igraph"
 defines ex_graph_def: "ex_graph \<equiv> Lgraph 
      {(home, cloud), (sphone, cloud), (cloud,hospital)}
@@ -77,7 +89,7 @@ defines ex_graph''_def: "ex_graph'' \<equiv> Lgraph
      ex_creds ex_locs"
 
 (* Same as above: the nicer representation with case suffers from
-   not so nice presentation in the cases (need to unfold the syntax) *) 
+   not so nice presentation in the cases (need to unfold the syntax) 
 fixes local_policies_alt :: "[igraph, location] \<Rightarrow> policy set"
 defines local_policies_alt_def: "local_policies_alt G \<equiv> 
     (\<lambda> x. case x of 
@@ -88,8 +100,7 @@ defines local_policies_alt_def: "local_policies_alt G \<equiv>
                 {((\<lambda> y. (\<exists> n. (n  @\<^bsub>G\<^esub> hospital) \<and> Actor n = y \<and> 
                            has G (y, ''skey''))), {put,get,move,eval})} 
        | _ \<Rightarrow>  {})"
-
-
+*)
 fixes local_policies :: "[igraph, location] \<Rightarrow> policy set"
 defines local_policies_def: "local_policies G \<equiv> 
     (\<lambda> x. if x = home then
@@ -121,7 +132,6 @@ defines Igdpr_def:
   "Igdpr \<equiv> {gdpr_scenario}"
 
 (* other states of scenario *)
-
 (* First step: Patient goes onto cloud *)
 fixes gdpr_scenario' :: "infrastructure"
 defines gdpr_scenario'_def:
@@ -150,7 +160,24 @@ fixes sgdpr
 defines "sgdpr \<equiv> {x. \<not> (global_policy' x ''Eve'')}"  
   
 begin
+subsection \<open>Using Attack Tree Calculus\<close>
+text \<open>Since we consider a predicate transformer semantics, we use sets of states 
+     to represent properties. For example, the attack property is given by the above
+     @{text \<open>set sgdpr\<close>}.
 
+The attack we are interested in is to see whether for the scenario
+
+@{text \<open>gdpr scenario \<equiv> Infrastructure ex_graph local_policies\<close>}
+
+from the initial state 
+
+@{text \<open>Igdpr \<equiv>{gdpr scenario}\<close>}, 
+
+the critical state
+@{text \<open>sgdpr\<close>} can be reached, i.e., is there a valid attack @{text \<open>(Igdpr,sgdpr)\<close>}?
+
+We first present a number of lemmas showing single and multi-step state transitions
+for relevant states reachable from our @{text \<open>gdpr_scenario\<close>}.\<close>
 lemma step1: "gdpr_scenario  \<rightarrow>\<^sub>n gdpr_scenario'"
 proof (rule_tac l = home and a = "''Patient''" and l' = cloud in move)
   show "graphI gdpr_scenario = graphI gdpr_scenario" by (rule refl)
@@ -218,6 +245,16 @@ qed
    impersonating the Doctor, for example). Insider attacks can
    be checked using the UasI predicate.
 *)
+text \<open>For the Kripke structure
+
+@{text \<open>gdpr_Kripke \<equiv> Kripke { I. gdpr_scenario \<rightarrow>\<^sub>i* I } {gdpr_scenario}\<close>}
+
+we first derive a valid and-attack using the attack tree proof calculus.
+
+@{text \<open>"\<turnstile>[\<N>\<^bsub>(Igdpr,GDPR')\<^esub>, \<N>\<^bsub>(GDPR',sgdpr)\<^esub>] \<oplus>\<^sub>\<and>\<^bsup>(Igdpr,sgdpr)\<^esup>\<close>}
+
+The set @{text \<open>GDPR'\<close>} (see above) is an intermediate state where Eve accesses the cloud.\<close>
+
 lemma gdpr_ref: "[\<N>\<^bsub>(Igdpr,sgdpr)\<^esub>] \<oplus>\<^sub>\<and>\<^bsup>(Igdpr,sgdpr)\<^esup> \<sqsubseteq>
                   [\<N>\<^bsub>(Igdpr,GDPR')\<^esub>, \<N>\<^bsub>(GDPR',sgdpr)\<^esub>] \<oplus>\<^sub>\<and>\<^bsup>(Igdpr,sgdpr)\<^esup>"  
 proof (rule_tac l = "[]" and l' = "[\<N>\<^bsub>(Igdpr,GDPR')\<^esub>, \<N>\<^bsub>(GDPR',sgdpr)\<^esub>]" and
@@ -249,6 +286,13 @@ lemma gdpr_abs_att: "\<turnstile>\<^sub>V [\<N>\<^bsub>(Igdpr,sgdpr)\<^esub>] \<
 proof (rule ref_valI, rule gdpr_ref, rule att_gdpr)
 qed
 
+text \<open>We can then simply apply the Correctness theorem @{text \<open>AT EF\<close>} to immediately 
+      prove the following CTL statement.
+
+      @{text \<open>gdpr_Kripke \<turnstile> EF sgdpr\<close>}
+
+This application of the meta-theorem of Correctness of attack trees saves us
+proving the CTL formula tediously by exploring the state space.\<close>
 lemma gdpr_att: "gdpr_Kripke \<turnstile> EF {x. \<not>(global_policy' x ''Eve'')}"
 proof -
   have a: " \<turnstile>[\<N>\<^bsub>(Igdpr, GDPR')\<^esub>, \<N>\<^bsub>(GDPR', sgdpr)\<^esub>] \<oplus>\<^sub>\<and>\<^bsup>(Igdpr, sgdpr)\<^esup>"
@@ -267,7 +311,8 @@ theorem gdpr_EF: "gdpr_Kripke \<turnstile> EF sgdpr"
 proof (insert gdpr_att, simp add: sgdpr_def)
 qed
 
-(* The CTL statement can now be directly translated into Attack Trees *)  
+text \<open>Similarly, vice-versa, the CTL statement can now be directly translated into
+    Attack Trees using the Completeness Theorem.\<close>
 theorem gdpr_AT: "\<exists> A. \<turnstile> A \<and> attack A = (Igdpr,sgdpr)"
 proof -
   have a: "gdpr_Kripke \<turnstile> EF sgdpr " by (rule gdpr_EF)
@@ -297,7 +342,35 @@ qed
    possible any more: gdpr_EF is not true any more *)  
   
 (** GDPR properties  for the illustration of the DLM labeling **)    
+section \<open>Data Protection by Design for GDPR compliance\<close>
+subsection \<open>General Data Protection Regulation (GDPR)\<close>
+text \<open>Since 26th May 2018, the GDPR has become mandatory within the European Union and hence 
+also for any supplier of IT products. Breaches of the regulation will be fined with penalties 
+of 20 Million EUR. Despite the relatively large size of the document of 209 pages, the technically 
+relevant portion for us is only about 30 pages (Pages 81–111, Chapters I to Chapter III, Section 3). 
+In summary, Chapter III specifies that the controller must give the data subject read access (1) 
+to any information, communications, and “meta-data” of the data, e.g., retention time and purpose. 
+In addition, the system must enable deletion of data (2) and restriction of processing.
+An invariant condition for data processing resulting from these Articles is that the system functions 
+must preserve any of the access rights of personal data (3).
 
+Using labeled data, we can now express the essence of Article 4 Paragraph (1): 
+’personal data’ means any information relating to an identified or identifiable natural 
+person (’data subject’).
+
+The labels of data must not be changed by processing: we have identified this  as 
+an invariant (3) resulting from the GDPR above. This invariant is formalized in 
+our Isabelle model by the type definition of functions on labeled data @{text \<open>label_fun\<close>}
+(see Section 4.2) that preserve the data labels.\<close>
+
+subsection \<open>Policy enforcement and privacy preservation\<close>
+text \<open>We can now use the labeled data to encode the privacy constraints of the 
+    GDPR in the rules. For example, the get data rule (see Section 4.3) has labelled data 
+    @{text \<open>((Actor a’, as), n)\<close>} and uses the labeling in the precondition to guarantee 
+    that only entitled users can get data.
+
+We can prove that processing preserves ownership as defined in the initial state for all paths 
+globally (AG) within the Kripke structure and in all locations of the graph.\<close>
 (* GDPR three: Processing preserves ownership in any location *)    
 lemma gdpr_three: "h \<in> gdpr_actors \<Longrightarrow> l \<in> gdpr_locations \<Longrightarrow>
          owns (Igraph gdpr_scenario) l (Actor h) d \<Longrightarrow>
@@ -319,8 +392,13 @@ next show "h \<in> gdpr_actors \<Longrightarrow>
       by (simp add: gdpr_scenario_def owns_def)
   qed
 
-(* Application example of Correctness and Completeness: 
-   show that there is no attack to ownership possible *)  
+text \<open>The final application example of Correctness contraposition 
+   shows that there is no attack to ownership possible.
+The proved meta-theory for attack trees can be applied to facilitate the proof. 
+The contraposition of the Correctness property grants that if there is no attack on 
+@{text \<open>(I,\<not>f)\<close>}, then @{text \<open>(EF \<not>f)\<close>} does not hold in the Kripke structure. This 
+yields the theorem since the @{text \<open>AG f\<close>} statement corresponds to @{text \<open>\<not>(EF \<not>f)\<close>}.
+\<close>
 theorem no_attack_gdpr_three: 
 "h \<in> gdpr_actors \<Longrightarrow> l \<in> gdpr_locations \<Longrightarrow> 
  owns (Igraph gdpr_scenario) l (Actor h) d \<Longrightarrow>
@@ -341,4 +419,5 @@ proof (rule_tac I = Igdpr and
     by (simp add: gdpr_Kripke_def Igdpr_def gdpr_states_def)
 qed
   
+end
 end
